iris/LinkPrputc.v
@@ -81,7 +81,7 @@ Section LinkPrputc.
               n eb b p lks HK Ha0 Hn Hbelow
               with "Hcg Hcpu Htext Hpc Huinv Hbase Htxl []").
     { iApply store_chain_of_out_chain.
-      iApply (out_chain_triv Uart1 _ emp%I eq_refl). done. }
+      iApply (out_chain_triv Uart1 _ _ emp%I eq_refl). done. }
     iIntros (CID1 Hs1 mf) "Hcg Hcpu Hpc %Hcs _".
     iSpecialize ("Hcont" $! CID1 with "[%]"); [exact Hs1|].
     iApply ("Hcont" $! mf with "Hcg Hcpu Hpc [%]"). exact Hcs.
